CollapsingTowers/TwoLevelMut/Defs.lean
@@ -1,2 +1,3 @@
 import CollapsingTowers.TwoLevelMut.Utils.Defs
 import CollapsingTowers.TwoLevelMut.Syntax.Defs
+import CollapsingTowers.TwoLevelMut.OperationalSemantics.Defs
